backend/Renumberproof.v
@@ -60,15 +60,24 @@ Proof.
   destruct f; reflexivity.
 Qed.
 
-Lemma find_function_translated:
-  forall ros rs fd,
-  find_function ge ros rs = Some fd ->
-  find_function tge ros rs = Some (transf_fundef fd).
+Lemma find_block_translated:
+  forall ros rs,
+    find_block tge ros rs = find_block ge ros rs.
 Proof.
-  unfold find_function; intros. destruct ros as [r|id].
-  eapply functions_translated; eauto.
-  rewrite symbols_preserved. destruct (Genv.find_symbol ge id); try congruence.
-  eapply function_ptr_translated; eauto.
+  unfold find_block; intros. destruct ros as [r|id]; auto.
+  apply symbols_preserved.
+Qed.
+
+Lemma find_function_translated:
+  forall ros rs fd fb,
+  find_block ge ros rs = Some fb ->
+  Genv.find_funct_ptr ge fb = Some fd ->
+  find_block tge ros rs = Some fb /\
+  Genv.find_funct_ptr tge fb = Some (transf_fundef fd).
+Proof.
+  intros.
+  exploit function_ptr_translated; eauto.
+  rewrite find_block_translated. auto.
 Qed.
 
 (** Effect of an injective renaming of nodes on a CFG. *)
@@ -146,10 +155,11 @@ Inductive match_states: RTL.state -> RTL.state -> Prop :=
         (REACH: reach f pc),
       match_states (State stk f sp pc rs m)
                    (State stk' (transf_function f) sp (renum_pc (pnum f) pc) rs m)
-  | match_callstates: forall stk f args m stk'
+  | match_callstates: forall stk f args m stk' b
+        (FIND: Genv.find_funct_ptr ge b = Some f)
         (STACKS: list_forall2 match_frames stk stk'),
-      match_states (Callstate stk f args m)
-                   (Callstate stk' (transf_fundef f) args m)
+      match_states (Callstate stk b args m)
+                   (Callstate stk' b args m)
   | match_returnstates: forall stk v m stk'
         (STACKS: list_forall2 match_frames stk stk'),
       match_states (Returnstate stk v m)
@@ -183,16 +193,16 @@ Proof.
   constructor; auto. eapply reach_succ; eauto. simpl; auto.
 (* call *)
   econstructor; split.
+  exploit find_function_translated; eauto. intros (FB & FIND).
   eapply exec_Icall with (fd := transf_fundef fd); eauto.
-    eapply find_function_translated; eauto.
     apply sig_preserved.
-  constructor. constructor; auto. constructor. eapply reach_succ; eauto. simpl; auto.
+  econstructor. eauto. constructor; auto. constructor. eapply reach_succ; eauto. simpl; auto.
 (* tailcall *)
   econstructor; split.
+  exploit find_function_translated; eauto. intros (FB & FIND).
   eapply exec_Itailcall with (fd := transf_fundef fd); eauto.
-    eapply find_function_translated; eauto.
     apply sig_preserved.
-  constructor. auto.
+  econstructor; eauto.
 (* builtin *)
   econstructor; split.
   eapply exec_Ibuiltin; eauto.
@@ -215,11 +225,15 @@ Proof.
   eapply exec_Ireturn; eauto.
   constructor; auto.
 (* internal function *)
+  rewrite FIND in H; inv H.
   simpl. econstructor; split.
-  eapply exec_function_internal; eauto.
-  constructor; auto. unfold reach. constructor.
+  apply function_ptr_translated in FIND.
+  eapply exec_function_internal; eauto. 
+  econstructor; eauto. unfold reach. constructor.
 (* external function *)
+  rewrite FIND in H; inv H.
   econstructor; split.
+  apply function_ptr_translated in FIND.
   eapply exec_function_external; eauto.
     eapply external_call_symbols_preserved; eauto. apply senv_preserved.
   constructor; auto.
@@ -240,7 +254,7 @@ Proof.
     rewrite symbols_preserved. rewrite (match_program_main TRANSL). eauto.
     eapply function_ptr_translated; eauto.
     rewrite <- H3; apply sig_preserved.
-  constructor. constructor.
+  econstructor. eauto. constructor.
 Qed.
 
 Lemma transf_final_states:
